Add hcall_tac

examples/delayed_echo/Echo01proof.v
@@ -204,27 +204,74 @@ End SOLVER.
 
 
 (******** TODO : remove redundancy with LL01proof ***********)
+Definition __gwf_mark__ (* (is_src: bool) *) (P: Prop): Prop := P.
+Lemma gwf_mark_spec: forall P, P <-> __gwf_mark__ P. refl. Qed.
+(* Opaque __gwf_mark__. *)
+Notation "'☀'" := (__gwf_mark__ _) (at level 60).
+
+
+
+(* Ltac iCheckWf := *)
+(*   tryif (match goal with | [WF0: URA.wf _, WF1: URA.wf _ |- _ ] => idtac end) then fail 1 else idtac *)
+(* . *)
+
+(* Ltac iClears' := *)
+(*   match goal with *)
+(*   | [ |- (gpaco3 (_sim_itree _) _ _ _ _ (([(_, (?src0, _))], ?src1), ?src2) (([(_, (?tgt0, _))], ?tgt1), ?tgt2)) ] => *)
+(*     let name := fresh "tmp" in *)
+(*     let all := constr:(src0 ⋅ src1 ⋅ tgt0 ⋅ tgt1) in *)
+(*     pose all as name; *)
+(*     repeat multimatch goal with *)
+(*            | [WF: URA.wf ?rh |- _ ] => tryif r_contains rh all then idtac else clear WF *)
+(*            | [H: iHyp ?ph ?rh |- _ ] => *)
+(*              tryif r_contains rh all then idtac else clear H *)
+(*                                                            (* idtac H; *) *)
+(*                                                            (*   idtac rh; *) *)
+(*                                                            (*   tryif r_contains rh all then idtac "CONTAINS" else idtac "DROP" *) *)
+(*            end; *)
+(*     clear name *)
+(*   end; *)
+(*   iCheckWf *)
+(* . *)
 Ltac iCheckWf :=
-  tryif (match goal with | [WF0: URA.wf _, WF1: URA.wf _ |- _ ] => idtac end) then fail 1 else idtac
+  (* tryif (match goal with | [WF0: __gwf_mark__ (URA.wf _), WF1: __gwf_mark__ (URA.wf _) |- _ ] => idtac end) then fail 1 else idtac *)
+  tryif (match goal with | [WF0: context[(URA.wf _)], WF1: context[(URA.wf _)] |- _ ] => idtac end) then fail 1 else idtac
 .
 
 Ltac iClears' :=
   match goal with
-  | [ |- (gpaco3 (_sim_itree _) _ _ _ _ (([(_, (?src0, _))], ?src1), ?src2) (([(_, (?tgt0, _))], ?tgt1), ?tgt2)) ] =>
-    let name := fresh "tmp" in
-    let all := constr:(src0 ⋅ src1 ⋅ tgt0 ⋅ tgt1) in
-    pose all as name;
+  | [ WF: __gwf_mark__ (URA.wf ?rs) |- _ ] =>
     repeat multimatch goal with
-           | [WF: URA.wf ?rh |- _ ] => tryif r_contains rh all then idtac else clear WF
            | [H: iHyp ?ph ?rh |- _ ] =>
-             tryif r_contains rh all then idtac else clear H
-                                                           (* idtac H; *)
-                                                           (*   idtac rh; *)
-                                                           (*   tryif r_contains rh all then idtac "CONTAINS" else idtac "DROP" *)
-           end;
-    clear name
+             tryif r_contains rh rs then idtac else clear H
+           end
   end;
-  iCheckWf
+  iCheckWf.
+
+Ltac iRefresh :=
+  clear_bar;
+  bar;
+  repeat multimatch goal with
+         | [H: URA.extends ?a ?b |- _ ] => replace (URA.extends a b) with ((Own a) b) in H by reflexivity
+         | [H: iHyp _ _ |- _ ] => revert H
+         (*** TODO: move existing resources to top ***)
+         (*** TODO: remove redundant URA.wf ***)
+         | [H: ?ip ?r |- _ ] =>
+           match type of ip with
+           | iProp => rewrite intro_iHyp in H; move r at top; move H at bottom
+           | _ => idtac
+           end
+         end;
+  i;
+  try (match goal with
+       | [ |- ?ip ?r ] =>
+         match type of ip with
+         | iProp => rewrite intro_iHyp
+         | _ => idtac
+         end
+       end;
+       iClears;
+       iClears')
 .
 
 Ltac iSplitP :=
@@ -263,18 +310,17 @@ Ltac iExists' Hs := let rs := r_gather Hs in exists rs.
 
 
 
+
+
+
+
 Require Import HTactics.
+Ltac harg_tac :=
+  HTactics.harg_tac;
+  match goal with
+  | [H: URA.wf _ |- _] => rewrite (gwf_mark_spec) in H
+  end.
 
-(* Definition __gwf_mark__ (P: Prop): Prop := P. *)
-(* Lemma gwf_mark_spec: forall P, P <-> __gwf_mark__ P. refl. Qed. *)
-(* Opaque __gwf_mark__. *)
-(* Notation "'☀'" := (__gwf_mark__ _) (at level 60). *)
-
-(* Ltac harg_tac := *)
-(*   HTactics.harg_tac; *)
-(*   match goal with *)
-(*   | [H: URA.wf _ |- _] => apply gwf_mark_spec in H *)
-(*   end. *)
 
 
 
@@ -366,15 +412,19 @@ Section SIMMODSEM.
   Opaque points_to.
 
   Lemma own_update: forall (x y: Σ) rx ctx, URA.updatable x y -> iHyp (Own x) rx -> URA.wf (rx ⋅ ctx) ->
-                                                   exists ry, iHyp (Own y) ry /\ URA.wf (ry ⋅ ctx) /\ URA.updatable rx ry.
+                                                   (* exists ry, iHyp (Own y) ry /\ URA.wf (ry ⋅ ctx) /\ URA.updatable rx ry. *)
+                                                   exists ry, iHyp (Own y) ry /\ URA.wf (ry ⋅ ctx) /\ URA.updatable (rx ⋅ ctx) (ry ⋅ ctx).
   Proof.
     { clear_until Σ. i. dup H. rr in H0. destruct H0; clear H0. subst. r in H.
       specialize (H (x0 ⋅ ctx)). rewrite ! URA.add_assoc in H. spc H.
       exists (y ⋅ x0). esplits; et.
       - rr. esplits; et.
-      - eapply URA.updatable_add; try refl. et.
+      - eapply URA.updatable_add; try refl. eapply URA.updatable_add; try refl. et.
     }
   Qed.
+
+  Ltac on_wf TAC := match goal with | WF:☀ |- _ => TAC WF end.
+
 
 
 
@@ -417,17 +467,48 @@ Section SIMMODSEM.
       steps. unfold hcall, ccall. steps.
       unfold body_to_tgt. unfold interp_hCallE_tgt, APC. steps. (********** TODO: never unfold it, make a lemma ******************)
       force_l; stb_tac; clarify. steps. rewrite Any.upcast_downcast. steps.
-      eapply hcall_clo; try lia; ss; et.
-      { let tmp := r_gather PRE in instantiate (1:=tmp).
-        instantiate (1:=ε).
-        let tmp := r_gather (A, A0) in instantiate (1:=tmp).
-        eapply URA.extends_updatable. r_equalize; r_solve. }
+      Inductive ltac_Wild : Set :=
+      | ltac_wild : ltac_Wild.
+      Notation "'__'" := ltac_wild : ltac_scope.
+      Open Scope ltac_scope.
+      
+      Ltac r_gather Hs :=
+        match Hs with
+        | (?H0, ?H1) => let rs0 := r_gather H0 in
+                        let rs1 := r_gather H1 in
+                        constr:((rs0 ⋅ rs1))
+        | ?H => match type of H with
+                | iHyp _ ?rh => constr:(rh)
+                | _ => H
+                end
+        end.
+      Ltac hcall_tac x o MR_SRC1 FR_SRC1 RARG_SRC :=
+        let mr_src1 := r_gather MR_SRC1 in
+        let fr_src1 := r_gather FR_SRC1 in
+        let rarg_src := r_gather RARG_SRC in
+        let tac0 := first [eapply URA.extends_updatable; r_equalize; r_solve (*** normal case ***)
+                          |rewrite ! URA.add_assoc in *; etrans; eauto; eapply URA.extends_updatable; r_equalize; r_solve
+(*** we have updatable in premise; TODO: do it better ***)] in
+        let tac1 := (on_wf ltac:(fun H => clear H);
+                     let WF := fresh "WF" in
+                     intros ? ? ? ? ? WF; cbn in WF; desH WF; subst;
+                     esplits; ss; et; i; rewrite gwf_mark_spec with (P:=URA.wf _) in *; iRefresh; iClears') in
+        prep;
+        match x with
+        | ltac_wild =>
+          match o with
+          | ltac_wild => eapply (hcall_clo _ (mr_src1:=mr_src1) (fr_src1:=fr_src1) (rarg_src:=rarg_src)); [tac0|lia|..|tac1]
+          | _ => eapply (hcall_clo _ (o:=o) (mr_src1:=mr_src1) (fr_src1:=fr_src1) (rarg_src:=rarg_src)); [tac0|lia|..|tac1]
+          end
+        | _ => eapply (hcall_clo x (o:=o) (mr_src1:=mr_src1) (fr_src1:=fr_src1) (rarg_src:=rarg_src)); [tac0|lia|..|tac1]
+        end
+      .
+      hcall_tac __ __ (A, A0) PRE (@URA.unit Σ); ss; et.
       { esplits; ss; et. eexists; iRefresh. left; iRefresh. iSplitL A; ss.
         - iApply A; ss.
         - iApply A0; ss.
       }
-      i; des; subst. esplits; ss; eauto. i; des; subst. iRefresh. iClears'.
-      rewrite Any.upcast_downcast. steps. rewrite Any.upcast_downcast. steps.
+      des; subst. rewrite Any.upcast_downcast. steps. rewrite Any.upcast_downcast. steps.
 
 
 
@@ -456,14 +537,11 @@ Section SIMMODSEM.
       destruct (dec z (- 1)%Z).
       - subst. ss. steps.
         force_l; stb_tac; clarify. steps. rewrite Any.upcast_downcast. steps.
-        eapply hcall_clo with (o:=ord_top); try lia; ss; et.
-        { instantiate (1:=ε).
-          let tmp := r_gather (PRE) in instantiate (1:=tmp).
-          let tmp := r_gather (A, SIM) in instantiate (1:=tmp).
-          eapply URA.extends_updatable. r_equalize; r_solve. }
+        hcall_tac __ __ (A, SIM) (@URA.unit Σ) PRE; ss; et.
         { esplits; try refl; iRefresh. iSplitP; ss. iSplitP; ss. }
+        { esplits; ss; et. }
         { esplits; ss; et. exists ns0; iRefresh. left; iRefresh. iSplit SIM A; ss. r_solve. }
-        i; des; subst. esplits; ss; eauto. i; des; subst. iRefresh. iClears'. steps.
+        steps.
         hret_tac mr (@URA.unit Σ); ss.
         { eapply URA.extends_updatable. esplit. r_equalize; r_solve. }
         { iRefresh. iDestruct SIM0. esplits; eauto. eexists; iRefresh. eauto. }
@@ -472,21 +550,14 @@ Section SIMMODSEM.
 
         rewrite unfold_APC. steps. force_l. exists false. steps. force_l. eexists ("push", [ll0; Vint z]↑). steps.
         force_l; stb_tac; clarify. steps. rewrite Any.upcast_downcast. steps.
-        eapply hcall_clo with (o:=ord_pure 2); try lia; ss; et.
-        { let tmp := r_gather (SIM) in instantiate (1:=tmp).
-          let tmp := r_gather (A) in instantiate (1:=tmp).
-          let tmp := r_gather (PRE) in instantiate (1:=tmp).
-          eapply URA.extends_updatable. r_equalize; r_solve. }
+        hcall_tac __ (ord_pure 2) PRE SIM A; ss; et.
         { instantiate (1:=(_, _)). esplits; try refl; iRefresh. eexists; iRefresh. iSplitP; ss. iSplitP; ss. iApply A; ss. }
         { esplits; ss; et. exists ns0; iRefresh. right; iRefresh; ss. }
-        i; des; subst. esplits; ss; eauto. i; des; subst. iRefresh. iClears'. steps.
-        rewrite Any.upcast_downcast in *. clarify.
-        do 2 iDestruct POST0. iPure A. apply Any.upcast_inj in A. des; clarify.
+        des; iRefresh. do 2 iDestruct POST0. iPure A. subst. apply Any.upcast_inj in A. des; clarify.
         iDestruct SIM0. destruct SIM0; iRefresh.
         { exfalso. iDestruct H1; subst. iMerge H1 SIM. rewrite <- own_sep in H1. rewrite GRA.padding_add in H1.
           iOwnWf H1. clear - WF. apply GRA.padding_wf in WF. des. ss.
         }
-
 
 
         rename H1 into A. iMerge A SIM. rewrite <- own_sep in A. rewrite GRA.padding_add in A. rewrite URA.add_comm in A.
@@ -501,143 +572,136 @@ Section SIMMODSEM.
         }
         subst.
 
-        eapply own_update in A; cycle 1.
+        Ltac iUpdate H :=
+          eapply own_update in H;
+          [let wf := fresh "WF" in let upd := fresh "UPD" in destruct H as [? [H [wf upd]]]; on_wf ltac:(fun H => clear H); rewrite gwf_mark_spec in wf; iRefresh| |
+          on_wf ltac:(fun H => eapply wf_downward; [|exact H]); eexists ε; r_equalize; r_solve; fail]; cycle 1.
+        iUpdate A.
         { eapply GRA.padding_updatable. instantiate (1:= echo_black (z :: ns0) ⋅ echo_white (z :: ns0)).
           eapply URA.auth_update. rr. ii. des; ss. destruct ctx; ss; clarify.
         }
-        { eapply wf_downward; et. erewrite f_equal; try refl. sym. r_equalize; r_solve. }
-        des. iRefresh.
         rewrite <- GRA.padding_add in A. rewrite own_sep in A. iDestruct A. subst.
-        iClears'. (**********************FIXME**********************) Undo 1.
-        clear VALID.
-
 
 
         rewrite unfold_APC. steps.
-        force_l; stb_tac; clarify. steps. rewrite Any.upcast_downcast. steps.
-        eapply hcall_clo with (o:=ord_top); try lia; ss; et.
-        { instantiate (1:=ε).
-          let tmp := r_gather (A2) in instantiate (1:=tmp).
-          let tmp := r_gather (POST0, A) in instantiate (1:=tmp).
-          rewrite ! URA.add_assoc. rewrite URA.unit_id.
-          replace (mr ⋅ x0 ⋅ x7 ⋅ x8) with (mr ⋅ x0 ⋅ (x7 ⋅ x8)) by r_solve.
-          replace (x7 ⋅ x9 ⋅ x10) with ((x9 ⋅ x10) ⋅ x7) by r_solve.
-          eapply URA.updatable_add; et.
-          eapply URA.extends_updatable. r_equalize; r_solve. }
+        force_l; stb_tac; clarify. steps. rewrite Any.upcast_downcast in *. steps.
+
+        hcall_tac __ ord_top (POST0, A) (@URA.unit Σ) A0; ss; et.
         { esplits; try refl; iRefresh. iSplitP; ss. iSplitP; ss. }
         { esplits; ss; eauto. exists (z :: ns0); iRefresh. left; iRefresh. iSplit A POST0; ss; r_solve. }
-        i; des; subst. esplits; ss; eauto. i; des; subst. iRefresh. iClears'. steps.
+        steps.
         hret_tac mr0 (@URA.unit Σ); ss.
         { eapply URA.extends_updatable; et. r_equalize; r_solve. }
         { esplits; eauto. }
     }
     econs; ss.
-    { HoareDef.init.
-      unfold checkWf, forge, discard, put. steps.
-      unfold echo_finishF, echo_finish_body. steps.
-      iRefresh. do 2 iDestruct _ASSUME0. iPure A. iPure A0. clarify.
-      iDestruct SIM.
-      destruct SIM as [A|A]; iRefresh; cycle 1.
-      { exfalso. iMerge A _ASSUME0. rewrite <- own_sep in A. rewrite GRA.padding_add in A.
-        iOwnWf A. clear - WF. apply GRA.padding_wf in WF. des. ss.
-      }
+    { admit "TODO". }
+    (* { HoareDef.init. *)
+    (*   unfold checkWf, forge, discard, put. steps. *)
+    (*   unfold echo_finishF, echo_finish_body. steps. *)
+    (*   iRefresh. do 2 iDestruct _ASSUME0. iPure A. iPure A0. clarify. *)
+    (*   iDestruct SIM. *)
+    (*   destruct SIM as [A|A]; iRefresh; cycle 1. *)
+    (*   { exfalso. iMerge A _ASSUME0. rewrite <- own_sep in A. rewrite GRA.padding_add in A. *)
+    (*     iOwnWf A. clear - WF. apply GRA.padding_wf in WF. des. ss. *)
+    (*   } *)
 
 
 
-      iDestruct A. subst.
-      rename x into ns. rename x0 into ns0.
-      assert(ns = ns0).
-      { iMerge A _ASSUME0. rewrite <- own_sep in A. rewrite GRA.padding_add in A.
-        iOwnWf A. eapply GRA.padding_wf in WF. des. eapply URA.auth_included in WF. des.
-        clear - WF.
-        Local Transparent URA.add.
-        rr in WF. des. ss. des_ifs.
-        Local Opaque URA.add.
-      }
-      subst.
-
-
-
-
-      steps. unfold hcall, ccall. steps.
-      unfold body_to_tgt. unfold interp_hCallE_tgt, APC. steps. (********** TODO: never unfold it, make a lemma ******************)
-
-      destruct ns0; ss.
-      - steps. rewrite Any.upcast_downcast. ss. steps.
-        rewrite unfold_is_list in A0. iPure A0. subst. ss. steps.
-        force_l. esplit. force_l. eexists (_, _). steps. force_l. { refl. } steps. force_l. esplit. force_l; ss. steps.
-        force_l. esplit. force_l. { refl. } steps.
-        { unfold alist_add. esplits; ss; eauto. eexists; iRefresh. left; iRefresh. instantiate (1:=[]). ss. iSplitL A; ss. }
-      - steps. rewrite Any.upcast_downcast. ss. steps.
-        force_l. eexists 3. steps.
-
-
-        assert(T: is_zero ll = false).
-        { rewrite unfold_is_list in *. do 4 iDestruct A0. iPure A0. subst. ss. }
-        rewrite T. clear T.
-        steps.
-
-
-        (* rr in A0. rr in A. rr in _ASSUME0. *)
-        (*** x2 x1 x5 ***)
-
-        rewrite unfold_APC. steps. force_l. exists false. steps. force_l. eexists ("alloc", [Vint 1]↑). steps.
-        force_l; stb_tac; clarify. steps. rewrite Any.upcast_downcast. steps.
-        unfold HoareCall at 3, checkWf, forge, discard, put. steps. force_l. eexists (x5, x2 ⋅ x1). steps. force_l.
-        { rewrite URA.unit_idl. eapply URA.extends_updatable. r_equalize; r_solve. }
-        steps. force_l. eexists ε. steps. force_l. eexists _. steps. force_l. { rewrite URA.unit_idl. refl. } steps.
-        force_l. eexists 1. steps. force_l. esplits. steps. force_l. esplits. steps. force_l.
-        { esplits; try refl. esplits; ss. }
-        steps. force_l. { esplits; ss; try lia. } steps.
-        clear_until _ASSUME0.
-        gstep; econs; try apply Nat.lt_succ_diag_r; i; ss.
-        { unfold alist_add; ss. esplits; ss; eauto. exists (z :: ns0); iRefresh. right; iRefresh; ss. }
-        exists 400. des. clarify. unfold alist_add; cbn. steps.
-        des. clarify. rewrite Any.upcast_downcast in *. clarify. iRefresh. iClears'.
-
-        do 2 iDestruct _ASSUME2. iPure _ASSUME2. subst. apply Any.upcast_inj in _ASSUME2. des; clarify.
-        iDestruct SIM. destruct SIM as [B|B]; iRefresh.
-        { exfalso. iDestruct B; subst. iMerge B A. rewrite <- own_sep in B. rewrite GRA.padding_add in B.
-          iOwnWf B. clear - WF. apply GRA.padding_wf in WF. des. ss.
-        }
-        assert(x = z :: ns0).
-        { iMerge A B. rewrite <- own_sep in A. rewrite GRA.padding_add in A.
-          iOwnWf A. eapply GRA.padding_wf in WF. des. eapply URA.auth_included in WF. des.
-          clear - WF.
-          Local Transparent URA.add.
-          rr in WF. des. ss. des_ifs.
-          Local Opaque URA.add.
-        }
-        subst.
-        steps.
+    (*   iDestruct A. subst. *)
+    (*   rename x into ns. rename x0 into ns0. *)
+    (*   assert(ns = ns0). *)
+    (*   { iMerge A _ASSUME0. rewrite <- own_sep in A. rewrite GRA.padding_add in A. *)
+    (*     iOwnWf A. eapply GRA.padding_wf in WF. des. eapply URA.auth_included in WF. des. *)
+    (*     clear - WF. *)
+    (*     Local Transparent URA.add. *)
+    (*     rr in WF. des. ss. des_ifs. *)
+    (*     Local Opaque URA.add. *)
+    (*   } *)
+    (*   subst. *)
 
 
 
 
+    (*   steps. unfold hcall, ccall. steps. *)
+    (*   unfold body_to_tgt. unfold interp_hCallE_tgt, APC. steps. (********** TODO: never unfold it, make a lemma ******************) *)
 
+    (*   destruct ns0; ss. *)
+    (*   - steps. rewrite Any.upcast_downcast. ss. steps. *)
+    (*     rewrite unfold_is_list in A0. iPure A0. subst. ss. steps. *)
+    (*     force_l. esplit. force_l. eexists (_, _). steps. force_l. { refl. } steps. force_l. esplit. force_l; ss. steps. *)
+    (*     force_l. esplit. force_l. { refl. } steps. *)
+    (*     { unfold alist_add. esplits; ss; eauto. eexists; iRefresh. left; iRefresh. instantiate (1:=[]). ss. iSplitL A; ss. } *)
+    (*   - steps. rewrite Any.upcast_downcast. ss. steps. *)
+    (*     force_l. eexists 3. steps. *)
+
+
+    (*     assert(T: is_zero ll = false). *)
+    (*     { rewrite unfold_is_list in *. do 4 iDestruct A0. iPure A0. subst. ss. } *)
+    (*     rewrite T. clear T. *)
+    (*     steps. *)
+
+
+    (*     (* rr in A0. rr in A. rr in _ASSUME0. *) *)
+    (*     (*** x2 x1 x5 ***) *)
+
+    (*     rewrite unfold_APC. steps. force_l. exists false. steps. force_l. eexists ("alloc", [Vint 1]↑). steps. *)
+    (*     force_l; stb_tac; clarify. steps. rewrite Any.upcast_downcast. steps. *)
+    (*     unfold HoareCall at 3, checkWf, forge, discard, put. steps. force_l. eexists (x5, x2 ⋅ x1). steps. force_l. *)
+    (*     { rewrite URA.unit_idl. eapply URA.extends_updatable. r_equalize; r_solve. } *)
+    (*     steps. force_l. eexists ε. steps. force_l. eexists _. steps. force_l. { rewrite URA.unit_idl. refl. } steps. *)
+    (*     force_l. eexists 1. steps. force_l. esplits. steps. force_l. esplits. steps. force_l. *)
+    (*     { esplits; try refl. esplits; ss. } *)
+    (*     steps. force_l. { esplits; ss; try lia. } steps. *)
+    (*     clear_until _ASSUME0. *)
+    (*     gstep; econs; try apply Nat.lt_succ_diag_r; i; ss. *)
+    (*     { unfold alist_add; ss. esplits; ss; eauto. exists (z :: ns0); iRefresh. right; iRefresh; ss. } *)
+    (*     exists 400. des. clarify. unfold alist_add; cbn. steps. *)
+    (*     des. clarify. rewrite Any.upcast_downcast in *. clarify. iRefresh. iClears'. *)
+
+    (*     do 2 iDestruct _ASSUME2. iPure _ASSUME2. subst. apply Any.upcast_inj in _ASSUME2. des; clarify. *)
+    (*     iDestruct SIM. destruct SIM as [B|B]; iRefresh. *)
+    (*     { exfalso. iDestruct B; subst. iMerge B A. rewrite <- own_sep in B. rewrite GRA.padding_add in B. *)
+    (*       iOwnWf B. clear - WF. apply GRA.padding_wf in WF. des. ss. *)
+    (*     } *)
+    (*     assert(x = z :: ns0). *)
+    (*     { iMerge A B. rewrite <- own_sep in A. rewrite GRA.padding_add in A. *)
+    (*       iOwnWf A. eapply GRA.padding_wf in WF. des. eapply URA.auth_included in WF. des. *)
+    (*       clear - WF. *)
+    (*       Local Transparent URA.add. *)
+    (*       rr in WF. des. ss. des_ifs. *)
+    (*       Local Opaque URA.add. *)
+    (*     } *)
+    (*     subst. *)
+    (*     steps. *)
 
 
 
 
 
-        rewrite unfold_APC. steps. force_l. exists false. steps. force_l. eexists ("pop2", [ll; Vptr x0 0]↑). steps.
-        force_l; stb_tac; clarify. steps. rewrite Any.upcast_downcast. steps.
-        unfold HoareCall at 3, checkWf, forge, discard, put. steps. force_l. eexists (mr, x1 ⋅ x2 ⋅ x3 ⋅ x7). steps. force_l.
-        { eapply URA.extends_updatable. r_equalize; r_solve. }
-        steps. force_l. exists (x2 ⋅ x7). steps. force_l. eexists _. steps. force_l.
-        { symmetry. r_equalize; r_solve. } steps.
-        force_l. eexists (List.map Vint (z :: ns0), x0). steps. force_l. esplits. steps. force_l. esplits. steps. force_l.
-        { esplits; try refl; iRefresh. eexists; iRefresh. iSplitP; ss. iSplit A0 A1; ss.
-          - iSplitP; ss.
-          - eexists; iRefresh. iApply A1; ss. }
-        steps. force_l. { esplits; ss; try lia. } steps.
-        clear_until A.
-        gstep; econs; try apply Nat.lt_succ_diag_r; i; ss.
-        { unfold alist_add; ss. esplits; ss; eauto. exists (z :: ns0); iRefresh. right; iRefresh; ss. }
-        exists 400. des. clarify. unfold alist_add; cbn. steps.
-        des. clarify. rewrite Any.upcast_downcast in *. clarify. iRefresh. iClears'.
-        admit "TODO~~~~~~~~~~~~".
-    }
+
+
+
+
+
+    (*     rewrite unfold_APC. steps. force_l. exists false. steps. force_l. eexists ("pop2", [ll; Vptr x0 0]↑). steps. *)
+    (*     force_l; stb_tac; clarify. steps. rewrite Any.upcast_downcast. steps. *)
+    (*     unfold HoareCall at 3, checkWf, forge, discard, put. steps. force_l. eexists (mr, x1 ⋅ x2 ⋅ x3 ⋅ x7). steps. force_l. *)
+    (*     { eapply URA.extends_updatable. r_equalize; r_solve. } *)
+    (*     steps. force_l. exists (x2 ⋅ x7). steps. force_l. eexists _. steps. force_l. *)
+    (*     { symmetry. r_equalize; r_solve. } steps. *)
+    (*     force_l. eexists (List.map Vint (z :: ns0), x0). steps. force_l. esplits. steps. force_l. esplits. steps. force_l. *)
+    (*     { esplits; try refl; iRefresh. eexists; iRefresh. iSplitP; ss. iSplit A0 A1; ss. *)
+    (*       - iSplitP; ss. *)
+    (*       - eexists; iRefresh. iApply A1; ss. } *)
+    (*     steps. force_l. { esplits; ss; try lia. } steps. *)
+    (*     clear_until A. *)
+    (*     gstep; econs; try apply Nat.lt_succ_diag_r; i; ss. *)
+    (*     { unfold alist_add; ss. esplits; ss; eauto. exists (z :: ns0); iRefresh. right; iRefresh; ss. } *)
+    (*     exists 400. des. clarify. unfold alist_add; cbn. steps. *)
+    (*     des. clarify. rewrite Any.upcast_downcast in *. clarify. iRefresh. iClears'. *)
+    (*     admit "TODO~~~~~~~~~~~~". *)
+    (* } *)
   Unshelve.
     all: ss.
     all: try (by repeat econs; et).
